Rewrite everything with an explicit substitution type, start defining a bunch of lemmas.

DeBruijnSn/Basic.lean
@@ -1,33 +1,54 @@
 
+
+
 inductive Term : Type where
 | var : Nat → Term
 | app : Term → Term → Term
 | lam : Term → Term
 
--- Ok so let's have this be computational
--- We follow https://hal.science/hal-00384683/document
-def φ (j i : Nat) : Term → Term
-| .var n => if n < i then .var n else .var $ n + j
-| .app t u => .app (φ j i t) (φ j i u)
-| .lam t => .lam $ φ j (i+1) t
+inductive Ren : Type where
+| idR : Ren
+| compR : Ren → Ren → Ren
+| lift : Ren
+
+inductive Subst : Type where
+| idS : Subst
+| comp : Subst → Ren → Subst
+| cons : Term → Subst → Subst
+
+infix:40 " ∘ " => Subst.comp
+notation "↑" => Ren.lift
+infix:80 " ⬝ " => Subst.cons
 
 set_option hygiene false
 
 -- idk about these precedences
-notation " [ " i:max " / " u:60 " ] " t:60 => (subst i u t)
+notation t:60 " ⟨ " s:60 " ⟩ " => (subst s t)
 
-def subst (i : Nat) (u : Term) : Term → Term
-| .var n =>
-  if n < i then .var n
-  else if n = i then φ i 0 u
-  else .var $ n - 1
-| .app t₁ t₂ => .app ([i/u]t₁) ([i/u]t₂)
-| .lam t => .lam $ [(i+1)/u]t
+def renVar (n : Nat) : Ren → Nat
+| .idR => n
+| .compR ρ₁ ρ₂ => renVar (renVar n ρ₁) ρ₂
+| ↑ => n+1
+
+def renTerm (ρ : Ren) : Term → Term
+| .var n => .var $ renVar n ρ
+| .app t₁ t₂ => .app (renTerm ρ t₁) (renTerm ρ t₂)
+| .lam t => .lam (renTerm (.compR ρ ↑) t)
+
+def substVar (n : Nat) : Subst → Term
+| .idS => .var n
+| t ⬝ σ => if n = 0 then t else substVar (n-1) σ
+| .comp σ ρ => (renTerm ρ (substVar n σ))
+
+def subst (σ : Subst) : Term → Term
+| .var n => substVar n σ
+| .app t₁ t₂ => .app (t₁⟨σ⟩) (t₂⟨σ⟩)
+| .lam t => .lam (t⟨ (.var 0) ⬝ (σ ∘ ↑) ⟩)
 
 notation t:60 " ⟶ " t':60 => (Red t t')
 
 inductive Red : Term → Term → Type where
-| beta : (.app (.lam t) u) ⟶ [0/u]t
+| beta : (.app (.lam t) u) ⟶ t⟨u ⬝ .idS⟩
 | congApp₁ : t ⟶ t' → (.app t u) ⟶ (.app t' u)
 | congApp₂ : u ⟶ u' → (.app t u) ⟶ (.app t u')
 | congLam : t ⟶ t' → (.lam t) ⟶ (.lam t')
@@ -49,7 +70,7 @@ end
 
 -- Weak head expansion: a family of "necessary reductions for normalization"
 inductive WeakHeadExp : Term → Term → Term → Type where
-| headWH : WeakHeadExp (.app (.lam t) u) ([0/u]t) u
+| headWH : WeakHeadExp (.app (.lam t) u) (t⟨u⬝.idS⟩) u
 | appWH : WeakHeadExp t t' u → WeakHeadExp (.app t v) (.app t' v) u
 
 inductive SN : Term → Type where
@@ -64,9 +85,6 @@ infix:60 " ⇒ " => Ty.arrow
 
 notation "Ctx" => (List Ty)
 
-#check List.get?
-#print Option
-
 notation ctx:50 " ⊢ " t:50 " :+ " ty:50 => (TypeTerm ctx t ty)
 inductive TypeTerm : Ctx → Term → Ty → Type where
 | varTy : ∀ Γ A n, Γ.get? n = .some A →  Γ ⊢ .var n :+ A
@@ -78,3 +96,78 @@ notation "⟦" ty "⟧" => (interpTy ty)
 def interpTy : Ty → Term → Type
 | .base => SN
 | ty₁ ⇒ ty₂ => λ t ↦ ∀ u, ⟦ty₁⟧ u → ⟦ty₂⟧ (.app t u)
+
+def compRenL (ρ : Ren) (σ: Subst) : Subst :=
+match ρ, σ with
+| .idR, _ => σ
+| ↑, _⬝ σ' => σ'
+| .compR ρ₁ ρ₂, _ => compRenL ρ₁ (compRenL ρ₂ σ)
+| _, .idS => .comp .idS ρ
+| ρ, .comp σ' ρ' => .comp (compRenL ρ σ') ρ' --ugh
+
+def compSubst (σ τ : Subst) : Subst :=
+match σ, τ with
+| u⬝σ', τ => u⟨τ⟩ ⬝ (compSubst σ' τ)
+| .idS, _ => τ
+| _, .idS => σ
+| .comp σ' ρ, τ => compSubst σ' (compRenL ρ τ)
+
+theorem subst_var_comp : subst σ (substVar x τ) = substVar x (compSubst τ σ) :=
+by sorry
+
+theorem comp_assoc : t⟨compSubst σ (τ ∘ ρ)⟩ = t⟨(compSubst σ τ ∘ ρ)⟩ :=
+by
+  cases σ <;> simp [compSubst]
+  case comp => sorry
+  case cons t' σ' => sorry
+
+theorem subst_comp : t⟨σ⟩⟨τ⟩ = t⟨compSubst σ τ⟩ :=
+by
+  cases t <;> simp [subst]
+  case var => apply subst_var_comp
+  case app => constructor <;> apply subst_comp
+  case lam =>
+    rw [subst_comp]
+    simp [compSubst, subst, substVar, compRenL]
+    sorry
+
+theorem substShift : t⟨.var 0 ⬝ (σ ∘ ↑)⟩ = t⟨σ⟩ :=
+by
+  revert σ
+  cases t <;> simp [subst] <;> intros σ
+  case var => simp [substVar]; sorry
+  case app => sorry
+  case lam => sorry
+
+theorem substIdS : t⟨.idS⟩ = t :=
+by
+  cases t <;> simp [subst, substVar]
+  case app => constructor <;> apply substIdS
+  case lam => sorry
+
+theorem compSubstIdL : compSubst .idS σ = σ :=
+by
+  cases σ <;> simp [compSubst]
+
+theorem compSubstIdR : compSubst σ .idS = σ :=
+by
+  cases σ <;> simp [compSubst]
+  case cons =>
+    constructor
+    . simp [subst]
+    sorry
+
+theorem comp_lift : compSubst (.var 0 ⬝ (σ ∘ ↑)) (t ⬝ .idS) = t ⬝ σ :=
+by
+  simp [compSubst, compRenL, subst, substVar]
+  apply compSubstIdR
+
+theorem subst_subst : t⟨(.var 0 ⬝ (σ ∘ ↑))⟩⟨u⬝.idS⟩ = t⟨u⬝σ⟩ :=
+by
+  rw [subst_comp, comp_lift]
+
+theorem app_subst : (.app ((.lam t)⟨σ⟩) u) ⟶ t⟨u⬝σ⟩ :=
+by
+  rw [← subst_subst]
+  simp [subst]
+  apply Red.beta
